doc/coq/Syntax.v
@@ -454,6 +454,258 @@ Proof.
     rewrite eq_ctx_eq in EQ. apply H0 in EQ. inversion EQ.
 Qed.
 
+(* injection, deletion *)
+
+Fixpoint map_inject {T} (Cout : @dy_ctx T) (Cin : @dy_ctx T) :=
+  match Cin with
+  | [||] => [||]
+  | dy_c_lam x t C' =>
+    dy_c_lam x t (map_inject Cout C')
+  | dy_c_lete x t C' =>
+    dy_c_lete x t (map_inject Cout C')
+  | dy_c_letm M C' C'' =>
+    dy_c_letm M (Cout[|map_inject Cout C'|]) (map_inject Cout C'')
+  end.
+
+Definition inject_ctx {T} (Cout : @dy_ctx T) (Cin : @dy_ctx T) :=
+  Cout[|map_inject Cout Cin|].
+
+Fixpoint delete_prefix {T} `{Eq T} (Cout : @dy_ctx T) (Cin : @dy_ctx T) :=
+  match Cout, Cin with
+  | [||], Cin => Cin
+  | dy_c_lam x t Cout', dy_c_lam x' t' Cin'
+  | dy_c_lete x t Cout', dy_c_lete x' t' Cin' =>
+    if eq_eid x x' && eqb t t' then
+      delete_prefix Cout' Cin'
+    else Cin
+  | dy_c_letm M Cout' Cout'', dy_c_letm M' Cin' Cin'' =>
+    if eq_mid M M' && eq_ctx Cout' Cin' then
+      delete_prefix Cout'' Cin''
+    else Cin
+  | _, _ => Cin
+  end.
+
+Ltac intro_refl :=
+  assert (forall x, eq_eid x x = true) as eid_refl; [intros; apply eq_eid_eq; eauto|idtac];
+  assert (forall M, eq_mid M M = true) as mid_refl; [intros; apply eq_mid_eq; eauto|idtac];
+  assert (forall {T} `{Eq T} t, eqb t t = true) as t_refl; [intros; apply eqb_eq; eauto|idtac];
+  assert (forall {T} `{Eq T} C, eq_ctx C C = true) as ctx_refl; [intros; apply eq_ctx_eq; eauto|idtac].
+
+Lemma delete_prefix_eq :
+  forall {T} `{Eq T} (Cout Cin : dy_ctx),
+    delete_prefix Cout (Cout[|Cin|]) = Cin.
+Proof.
+  intro_refl. intros. rename H into ET. revert Cin.
+  induction Cout; simpl; eauto;    
+    try rewrite eid_refl; try rewrite mid_refl; try rewrite t_refl; try rewrite ctx_refl;
+    simpl; eauto.
+Qed.
+
+Lemma delete_prefix_dec :
+  forall {T} `{Eq T} (Cout Cin : @dy_ctx T),
+    dy_level (delete_prefix Cout Cin) <= dy_level Cin.
+Proof.
+  intros. revert Cout. 
+  induction Cin; intros; destruct Cout; simpl; eauto;
+  try destruct (eq_eid x0 x); try destruct (eqb tx0 tx);
+  try destruct (eq_mid M0 M); try destruct (eq_ctx Cout1 Cin1);
+  simpl; try nia.
+  etransitivity; try apply IHCin; eauto.
+  etransitivity; try apply IHCin; eauto.
+  etransitivity; try apply IHCin2; nia.
+Qed.
+
+Require Import Program.
+
+Program Fixpoint delete_map 
+  {T} `{Eq T} (Cout Cin : dy_ctx) {measure (dy_level Cin)} :=
+  match Cin with
+  | [||] => [||]
+  | dy_c_lam x t C' =>
+    dy_c_lam x t (delete_map Cout C')
+  | dy_c_lete x t C' =>
+    dy_c_lete x t (delete_map Cout C')
+  | dy_c_letm M C' C'' =>
+    dy_c_letm M (delete_map Cout (delete_prefix Cout C'))
+                (delete_map Cout C'')
+  end.
+
+Next Obligation.
+  simpl.
+  pose proof (delete_prefix_dec Cout C').
+  nia.
+Defined.
+Next Obligation.
+  simpl.
+  pose proof (delete_prefix_dec Cout C'').
+  nia.
+Defined.
+
+(* reduction lemmas *)
+Lemma delete_map_red_lam :
+  forall {T} `{Eq T} Cout x t C',
+    delete_map Cout (dy_c_lam x t C') =
+      dy_c_lam x t (delete_map Cout C').
+Proof.
+  intros. unfold delete_map. unfold delete_map_func.
+  rewrite fix_sub_eq; simpl; try reflexivity.
+  intros x' f g Heq.
+  specialize (functional_extensionality_dep f g Heq).
+  intros RR. rewrite RR. reflexivity.
+Qed.
+
+Lemma delete_map_red_lete :
+  forall {T} `{Eq T} Cout x t C',
+    delete_map Cout (dy_c_lete x t C') =
+      dy_c_lete x t (delete_map Cout C').
+Proof.
+  intros. unfold delete_map. unfold delete_map_func.
+  rewrite fix_sub_eq; simpl; try reflexivity.
+  intros x' f g Heq.
+  specialize (functional_extensionality_dep f g Heq).
+  intros RR. rewrite RR. reflexivity.
+Qed.
+
+Lemma delete_map_red_letm :
+  forall {T} `{Eq T} Cout M C' C'',
+    delete_map Cout (dy_c_letm M C' C'') =
+      dy_c_letm M (delete_map Cout (delete_prefix Cout C'))
+                  (delete_map Cout C'').
+Proof.
+  intros. unfold delete_map. unfold delete_map_func.
+  rewrite fix_sub_eq; simpl; try reflexivity.
+  intros x' f g Heq.
+  specialize (functional_extensionality_dep f g Heq).
+  intros RR. rewrite RR. reflexivity.
+Qed.
+
+Ltac simpl_delete :=
+  simpl;
+  try rewrite delete_map_red_lam;
+  try rewrite delete_map_red_lete;
+  try rewrite delete_map_red_letm.
+
+Lemma delete_map_eq :
+  forall {T} `{Eq T} (Cout Cin : dy_ctx),
+    delete_map Cout (map_inject Cout Cin) = Cin.
+Proof.
+  intros. rename H into ET. revert Cout.
+  induction Cin; intros; simpl_delete; 
+  try rewrite IHCin; eauto.
+  rewrite delete_prefix_eq. 
+  rewrite IHCin1. rewrite IHCin2. eauto.
+Qed.
+
+Definition delete_inject {T} `{Eq T} (Cout Cin : dy_ctx) :=
+  delete_map Cout (delete_prefix Cout Cin).
+
+Lemma delete_inject_eq :
+  forall {T} `{Eq T} (Cout Cin : dy_ctx),
+    delete_inject Cout (inject_ctx Cout Cin) = Cin.
+Proof.
+  intros. unfold delete_inject. unfold inject_ctx.
+  rewrite delete_prefix_eq.
+  rewrite delete_map_eq. eauto.
+Qed.
+  
+Notation "Cout '<|' Cin '|>'" := (inject_ctx Cout Cin)
+                              (at level 100, Cin at next level, right associativity).
+
+Definition inject_ctx_v {T} `{Eq T} (Cout : @dy_ctx T) (v : @expr_value T) :=
+  match v with
+  | Closure x t C => Closure x t (Cout <|C|>)
+  end.
+
+Definition delete_ctx_v {T} `{Eq T} (Cout : @dy_ctx T) (v : @expr_value T) :=
+  match v with
+  | Closure x t C => Closure x t (delete_inject Cout C)
+  end.
+
+Lemma map_inject_addr_x :
+  forall {T} `{Eq T} x (Cout : @dy_ctx T) (Cin : @dy_ctx T),
+    addr_x (map_inject Cout Cin) x = addr_x Cin x.
+Proof.
+  intros. revert Cout. 
+  induction Cin; intros; simpl; eauto;
+  destruct (addr_x Cin x) eqn:ADDR;
+  rewrite IHCin; eauto.
+Qed.
+
+Lemma map_inject_ctx_M :
+  forall {T} `{Eq T} M (Cout : @dy_ctx T) (Cin : @dy_ctx T),
+    ctx_M (map_inject Cout Cin) M =
+    match ctx_M Cin M with
+    | Some CM => Some (Cout <| CM |>)
+    | None => None
+    end.
+Proof.
+  intros. revert Cout.
+  induction Cin; intros; simpl; eauto.
+  rewrite IHCin2. destruct (ctx_M Cin2 M); eauto.
+  destruct (eq_mid M M0); eauto.
+Qed.
+
+Lemma plugin_ctx_addr_x :
+  forall {T} `{Eq T} x (Cout : @dy_ctx T) (Cin : @dy_ctx T),
+    match addr_x Cin x with
+    | Some t => addr_x (Cout[|Cin|]) x = Some t
+    | None => True
+    end.
+Proof.
+  intros. revert Cin.
+  induction Cout; intros; 
+  destruct (addr_x Cin x) eqn:ADDR; simpl; eauto;
+  try (specialize (IHCout Cin); rewrite ADDR in IHCout;
+      rewrite IHCout; eauto).
+  specialize (IHCout2 Cin); rewrite ADDR in IHCout2; rewrite IHCout2; eauto.
+Qed.
+
+Lemma plugin_ctx_ctx_M :
+  forall {T} `{Eq T} M (Cout : @dy_ctx T) (Cin : @dy_ctx T),
+    match ctx_M Cin M with
+    | Some CM => ctx_M (Cout[|Cin|]) M = Some CM
+    | None => True
+    end.
+Proof.
+  intros. revert Cin.
+  induction Cout; intros;
+  destruct (ctx_M Cin M) eqn:CTX; simpl; eauto;
+  try (specialize (IHCout Cin); rewrite CTX in IHCout;
+      rewrite IHCout; eauto).
+  specialize (IHCout2 Cin); rewrite CTX in IHCout2; rewrite IHCout2; eauto.
+Qed.
+
+Lemma inject_ctx_addr_x :
+  forall {T} `{Eq T} x (Cout : @dy_ctx T) (Cin : @dy_ctx T),
+    match addr_x Cin x with
+    | Some t => addr_x (Cout<|Cin|>) x = Some t
+    | None => True
+    end.
+Proof.
+  intros. destruct (addr_x Cin x) eqn:ADDR; eauto.
+  rewrite <- map_inject_addr_x with (Cout := Cout) in ADDR.
+  rewrite <- ADDR. 
+  pose proof plugin_ctx_addr_x.
+  specialize (H0 x Cout (map_inject Cout Cin)).
+  rewrite ADDR in H0. rewrite <- H0 in ADDR.
+  eauto.
+Qed.
+
+Lemma inject_ctx_ctx_M :
+  forall {T} `{Eq T} M (Cout : @dy_ctx T) (Cin : @dy_ctx T),
+    match ctx_M Cin M with
+    | Some CM => ctx_M (Cout<|Cin|>) M = Some (Cout <|CM|>)
+    | None => True
+    end.
+Proof.
+  intros. destruct (ctx_M Cin M) eqn:CTX; eauto.
+  pose proof (map_inject_ctx_M M Cout Cin).
+  rewrite CTX in H0.
+  pose proof (plugin_ctx_ctx_M M Cout (map_inject Cout Cin)).
+  rewrite H0 in H1. eauto.
+Qed.
+
+(* Typeclass for concrete times *)
 Class OrderT (T : Type) `{Eq T} : Type :=
 {
   leb : T -> T -> bool;
