doc/coq/ALinking.v
@@ -1,0 +1,131 @@
+From MODULAR Require Export Abstract.
+Require Export Coq.Logic.FunctionalExtensionality.
+
+Generalizable Variables T.
+
+Definition inject_ctx_mem `{Eq T} (Cout : @dy_ctx T) (mem : T -> list expr_value) :=
+  fun t => map (inject_ctx_v Cout) (mem t).
+
+Definition delete_ctx_mem `{Eq T} (Cout : @dy_ctx T) (mem : T -> list expr_value) :=
+  fun t => map (delete_ctx_v Cout) (mem t).
+
+Lemma delete_ctx_mem_eq :
+  forall `{Eq T} (Cout : @dy_ctx T) (mem : T -> list expr_value),
+         delete_ctx_mem Cout (inject_ctx_mem Cout mem) = mem.
+Proof.
+  intros. apply functional_extensionality.
+  intros. unfold inject_ctx_mem. unfold delete_ctx_mem.
+  remember (mem x) as l. clear Heql x mem. revert Cout.
+  induction l; try reflexivity. intros.
+  destruct a; simpl.
+  rewrite delete_inject_eq.
+  rewrite IHl. reflexivity.
+Qed.
+
+Definition delete_update `{time T} (Cout : @dy_ctx T) :=
+  fun C st x v =>
+    match st with
+    | ST mem t =>
+      update (delete_inject Cout C)
+             (ST (delete_ctx_mem Cout mem) t)
+             x (delete_ctx_v Cout v)
+    end.
+
+#[export] Instance delete_time `{time T} (Cout : @dy_ctx T) : time :=
+  {
+    update := delete_update Cout
+  }.
+
+Lemma delete_update_eq `{time T} (Cout : @dy_ctx T) :
+  forall C mem t x v,
+    delete_update Cout (Cout<|C|>) (ST (inject_ctx_mem Cout mem) t) x (inject_ctx_v Cout v) =
+    update C (ST mem t) x v.
+Proof.
+  intros. destruct v. unfold inject_ctx_v.
+  unfold delete_update. simpl.
+  rewrite delete_inject_eq. rewrite delete_ctx_mem_eq.
+  rewrite delete_inject_eq. reflexivity.
+Qed.
+
+Lemma plugin_map_assoc :
+  forall `{Eq T} (Cout C C' : @dy_ctx T),
+    (map_inject Cout C) [|map_inject Cout C'|] = (map_inject Cout (C [|C'|])).
+Proof.
+  intros. revert Cout C'. induction C; intros; simpl; eauto; try rewrite IHC; try rewrite IHC2; eauto.
+Qed.
+
+Lemma plugin_inject_assoc :
+  forall `{Eq T} (Cout C C' : @dy_ctx T),
+    (Cout <| C |>)[| map_inject Cout C' |] = (Cout <|C[|C'|]|>).
+Proof.
+  intros. unfold inject_ctx. rewrite <- c_plugin_assoc.
+  rewrite plugin_map_assoc. eauto.
+Qed.
+
+Lemma inject_update_m_eq :
+  forall `{Eq T} t x e mem (Cout C : @dy_ctx T),
+  (t !#-> Closure x e (Cout <| C |>); inject_ctx_mem Cout mem) =
+            inject_ctx_mem Cout (t !#-> Closure x e C; mem).
+Proof.
+  intros. apply functional_extensionality.
+  intros. unfold update_m. unfold inject_ctx_mem.
+  destruct (eqb x0 t); eauto.
+Qed.
+
+Lemma delete_eval_eq {T} `{ET : Eq T} `{TT : @time T ET} (Cout : @dy_ctx T) :
+  forall C st e v st'
+         (EVAL : @EvalR T ET TT C st e v st'),
+    let inject_v :=
+      match v with
+      | EVal (Closure x_v e_v C_v) => EVal (Closure x_v e_v (Cout<|C_v|>))
+      | MVal C_v => MVal (Cout<|C_v|>)
+      end in
+    let inject_st :=
+      match st with
+      | ST mem t => ST (inject_ctx_mem Cout mem) t
+      end in
+    let inject_st' :=
+      match st' with
+      | ST mem' t' => ST (inject_ctx_mem Cout mem') t'
+      end in
+    @EvalR T ET (@delete_time T ET TT Cout)
+      (Cout<|C|>) inject_st e inject_v inject_st'.
+Proof.
+  intros. induction EVAL;
+  try destruct v; try destruct st; try destruct st'; try destruct st'';
+  try (destruct inject_v eqn:INJv; inversion INJv; subst);
+  try (destruct inject_st eqn:INJst; inversion INJst; subst);
+  try (destruct inject_st' eqn:INJst'; inversion INJst'; subst); eauto.
+  - inversion STATE; subst.
+    eapply Eval_var_e; eauto.
+    pose proof (inject_ctx_addr_x x Cout C) as RR.
+    rewrite <- ADDR in RR. symmetry. apply RR.
+    unfold inject_ctx_mem. 
+    remember (mem0 addr) as l.
+    clear Heql C mem0 x addr t0 inject_st' INJst' STATE inject_st INJst ADDR inject_v INJv.
+    revert Cout x0 e C0 ACCESS. induction l; simpl; intros; eauto.
+    destruct ACCESS as [L | R].
+    left. rewrite L. simpl. eauto.
+    right. apply IHl. eauto.
+  - destruct st_v. destruct arg.
+    eapply Eval_app. apply IHEVAL1. apply IHEVAL2.
+    pose proof (delete_update_eq Cout C mem t x (Closure x1 e3 C1)) as RR.
+    simpl in *. rewrite RR. clear RR.
+    rewrite inject_update_m_eq.
+    replace (dy_c_lam x t ([||])) with (map_inject Cout (dy_c_lam x t ([||]))) by reflexivity.
+    rewrite plugin_inject_assoc. eauto.
+  - pose proof (inject_ctx_ctx_M M Cout C) as RR. 
+    rewrite <- ACCESS in RR.
+    eapply Eval_var_m; eauto.
+  - eapply Eval_lete; eauto.
+    pose proof (delete_update_eq Cout C mem t x (Closure x0 e0 C0)) as RR.
+    simpl in *. rewrite RR. clear RR.
+    rewrite inject_update_m_eq.
+    replace (dy_c_lete x t ([||])) with (map_inject Cout (dy_c_lete x t ([||]))) by reflexivity.
+    rewrite plugin_inject_assoc. eauto.
+  - eapply Eval_letm; eauto.
+    assert ((Cout <| C |>) [|dy_c_letm M (Cout <| C' |>) ([||])|] =
+            (Cout <| (C [|dy_c_letm M C' ([||])|]) |>)) as RR. 
+    { rewrite <- plugin_inject_assoc. simpl. eauto. } 
+    rewrite RR. clear RR. simpl in *. exact IHEVAL2.
+Qed.
